src/tutorial/PulseTutorial.MonotonicCounter.fst
@@ -35,7 +35,6 @@ let increases : preorder int = fun x y -> b2t (x <= y)
 let mctr = MR.mref increases
 
 fn new_counter ()
-requires emp
 returns c:ctr
 ensures c.inv 0
 {
@@ -63,9 +62,7 @@ ensures c.inv 0
         MR.recall_snapshot mr;
     };
     ghost
-    fn dup (#_:unit) : dup_f snapshot = i {
-        MR.dup_snapshot mr;
-    };
+    fn dup (#_:unit) : dup_f snapshot = i {};
     let c = { inv; snapshot; next; destroy; snap; recall; dup };
     rewrite (inv 0) as (c.inv 0);
     c
@@ -73,7 +70,8 @@ ensures c.inv 0
 
 
 fn do_something (c:ctr) (#i #k:erased int)
-requires c.inv i ** c.snapshot k
+requires c.inv i
+requires c.snapshot k
 ensures exists* j. c.inv j
 {
   let recall = c.recall;
@@ -82,8 +80,6 @@ ensures exists* j. c.inv j
 }
 
 fn test_counter ()
-requires emp
-ensures emp
 {
     let c = new_counter ();
     snap c;
